Add sections in Correctness; move cumulativity to Metatheory; update dependencies

Correctness.v
@@ -1,3 +1,16 @@
+(** Formalization of a Predicative System F
+
+In this file, we state and prove correctness (and sometimes
+completeness) properties about previously defined functions.
+More precisely, we prove:
+
+  * correctness for our decidable structural equality predicate
+    over types ;
+  * correctness and completeness for our decidable predicates
+    for the wellformedness of types and environments ;
+  * correctness for our kinding algorithm ;
+  * correctness for our typing algorithm. *)
+
 Require Import Arith.
 Require Import Arith.Max.
 Require Import Arith.Compare_dec.
@@ -7,159 +20,178 @@ Require Import Bool.
 
 Add LoadPath ".".
 
+(** Use [make SysF.vo Metatheory.vo] to compile the modules
+    before executing these lines. *)
 Require Import SysF.
+Require Import Metatheory. (* for cumulativity *)
 
-Lemma beq_typ_correct : forall T1 T2 : typ, beq_typ T1 T2 = true -> T1 = T2.
-  induction T1.
-  - intros.
-    destruct T2; [ auto using beq_nat_eq | inversion H .. ].
-  - intros.
-    destruct T2.
-    + inversion H.
-    + apply andb_true_iff in H. 
-      destruct H.
-      apply IHT1_1 in H.
-      apply IHT1_2 in H0. 
-      congruence.
-    + inversion H.
-  - intros.
-    destruct T2.
-    + inversion H.
-    + inversion H.
-    + apply andb_true_iff in H.
-      destruct H.
-      apply IHT1 in H0.
-      apply eq_sym in H. apply beq_nat_eq in H.
-      congruence.
-Qed.
+Section Equality.
 
-Lemma beq_typ_refl : forall T : typ, beq_typ T T = true.
-  intro.
-  induction T.
-  - apply eq_sym. apply beq_nat_refl.
-  - apply andb_true_iff. split. apply IHT1. apply IHT2.
-  - apply andb_true_iff. split. symmetry. apply beq_nat_refl. apply IHT.
-Qed.
+  (** This lemma states the correctness of beq_typ. That is, that
+      whenever beq_typ says two types are equal, they are indeed
+      equal. *)
+  Lemma beq_typ_correct : forall T1 T2 : typ,
+                            beq_typ T1 T2 = true -> T1 = T2.
+    induction T1.
+    - intros.
+      destruct T2; [ auto using beq_nat_eq | inversion H .. ].
+    - intros.
+      destruct T2.
+      + inversion H.
+      + apply andb_true_iff in H. 
+        destruct H.
+        apply IHT1_1 in H.
+        apply IHT1_2 in H0. 
+        congruence.
+      + inversion H.
+    - intros.
+      destruct T2.
+      + inversion H.
+      + inversion H.
+      + apply andb_true_iff in H.
+        destruct H.
+        apply IHT1 in H0.
+        apply eq_sym in H. apply beq_nat_eq in H.
+        congruence.
+  Qed.
 
-(* This is actually cumulativity *)
-Lemma kinding_sub : forall (e : env) (T : typ) (K : kind),
-                          kinding e T K -> forall K', K <= K' -> kinding e T K'.
-  do 4 intro.
-  induction H.
-  - intros.
-    assert (Kp <= K') by omega.
-    eauto using k_tvar.
-  - intros.
-    destruct K'.
-    + inversion H0.
-    + assert (max Kp Kq <= K') by omega.
-      assert (max K' Kq = K') by eauto with arith.
-      rewrite <- H2.
-      eauto using k_tall with arith.
-  - intros.
-    assert (Kp <= max Kp Kq /\ Kq <= max Kp Kq) by auto with arith.
-    assert (max K' K' = K') by auto with arith.
-    rewrite <- H3.
-    destruct H2.
-    apply k_tarr; [ eauto using le_trans .. ]. (* TODO just eauto using k_tarr, le_trans doesn't work *)
-Qed.
+  (** This lemma states the reflexivity of beq_typ. *)
+  Lemma beq_typ_refl : forall T : typ, beq_typ T T = true.
+    intro.
+    induction T.
+    - apply eq_sym. apply beq_nat_refl.
+    - apply andb_true_iff. split. apply IHT1. apply IHT2.
+    - apply andb_true_iff. split. symmetry. apply beq_nat_refl. apply IHT.
+  Qed.
 
-Definition cumulativity := kinding_sub.
+End Equality.
 
+Section Wellformedness.
 
-(* TODO simplified the equivalences to implications so this plays nice with eauto *)
-Lemma bwf_typ_correct : forall T : typ, forall e : env, bwf_typ e T = true -> wf_typ e T.
-  induction T.
-  - intro. simpl.
-    destruct (get_kind e n); [ intuition .. ]. discriminate.
-  - intros.
-    apply andb_true_iff in H.
-    split.
-    + apply IHT1. apply H.
-    + apply IHT2. apply H.
-  - intro. apply IHT.
-Qed.
+  (** This lemma states the correctness of bwf_typ. That is, that
+      whenever bwf_typ says a type is well formed, it is indeed
+      well formed. *)
+  (* TODO simplified the equivalences to implications so this plays nice with eauto *)
+  Lemma bwf_typ_correct : forall T : typ, forall e : env,
+                          bwf_typ e T = true -> wf_typ e T.
+    induction T.
+    - intro. simpl.
+      destruct (get_kind e n); [ intuition .. ]. discriminate.
+    - intros.
+      apply andb_true_iff in H.
+      split.
+      + apply IHT1. apply H.
+      + apply IHT2. apply H.
+    - intro. apply IHT.
+  Qed.
 
-Lemma bwf_typ_complete : forall (T : typ) (e : env), wf_typ e T -> bwf_typ e T = true.
-  induction T; simpl; auto; intros.
-  - destruct (get_kind e n); auto.
-  - apply andb_true_iff. split; [apply IHT1 | apply IHT2]; destruct H; auto.
-Qed. 
+  (** This lemma states the completeness of bwf_typ. That is, that
+      whenever a type is well formed, bwf_typ successfully says that
+      it is. *)
+  Lemma bwf_typ_complete : forall (T : typ) (e : env),
+                           wf_typ e T -> bwf_typ e T = true.
+    induction T; simpl; auto; intros.
+    - destruct (get_kind e n); auto.
+    - apply andb_true_iff. split; [apply IHT1 | apply IHT2]; destruct H; auto.
+  Qed. 
 
-Lemma bwf_env_correct : forall e : env, bwf_env e = true -> wf_env e.
-  induction e; simpl; auto.
-  - intro.
-    apply andb_true_iff in H.
-    split.
-    + apply bwf_typ_correct. apply H.
-    + apply IHe. apply H.
-Qed.
+  (** This lemma states the correctness of bwf_env. That is, that
+      whenever bwf_env says an environment is well formed, it is
+      indeed well formed. *)
+  Lemma bwf_env_correct : forall e : env,
+                            bwf_env e = true -> wf_env e.
+    induction e; simpl; auto.
+    - intro.
+      apply andb_true_iff in H.
+      split.
+      + apply bwf_typ_correct. apply H.
+      + apply IHe. apply H.
+  Qed.
 
-Lemma bwf_env_complete : forall e : env, wf_env e -> bwf_env e = true.
-  induction e; auto.
-  - intro. simpl. apply andb_true_iff. split; destruct H; auto using bwf_typ_complete.
-Qed.
+  (** This lemma states the completeness of bwf_env. That is, that
+      whenever an environment is well formed, bwf_env successfully says that
+      it is. *)
+  Lemma bwf_env_complete : forall e : env, wf_env e -> bwf_env e = true.
+    induction e; auto.
+    - intro. simpl. apply andb_true_iff. split; destruct H; auto using bwf_typ_complete.
+  Qed.
 
-Theorem kind_of_correct (T : typ) : 
-  forall (e : env) (K : kind), 
-    kind_of e T = Some K -> kinding e T K.
-  induction T.
-  - intros. simpl in H.
-    remember (bwf_env e).
-    destruct b.
-    + apply eq_sym in Heqb. eauto using bwf_env_correct, k_tvar.
-    + discriminate H.
-  - intros. simpl in H.
-    remember (kind_of e T1) as kind_of_T1.
-    remember (kind_of e T2) as kind_of_T2.
-    destruct kind_of_T1, kind_of_T2;
-      [ inversion H; eauto using k_tarr | inversion H .. ].
-  - intros. simpl in H.
-    destruct (kind_of (etvar k e) T) eqn:kind_of_etvar.
-    + inversion H. eauto using k_tall.
-    + inversion H.
-Qed. 
+End Wellformedness.
 
-Theorem type_of_correct (t : term) : 
-  forall (e : env) (T : typ), 
-    type_of e t = Some T -> typing e t T.
-  induction t.
-  - intros. simpl in H.
-    destruct (bwf_env e) eqn:env_is_bwf.
-    + auto using t_var, bwf_env_correct.
-    + inversion H.
-  - intros. simpl in H.
-    destruct (type_of (evar t e) t0) eqn:type_of_body.
-    + remember (bwf_typ e t). destruct b.
-      * inversion H. apply t_abs. apply bwf_typ_correct. auto. apply IHt, type_of_body.
-      * discriminate.
-    + inversion H.
-  - intros. simpl in H.
-    destruct (type_of e t1) eqn:type_of_fn.
-    + destruct t.
-      * inversion H.
-      * destruct (type_of e t2) eqn:type_of_arg.
-        { destruct (beq_typ t3 t) eqn:equal_types.
-          { inversion H. rewrite <- H1.
-            eauto. apply beq_typ_correct in equal_types. eapply t_app. eauto. rewrite equal_types. eauto. }
-          { inversion H. } }
-        { inversion H. }
-      * inversion H.
-    + inversion H.
-  - intros. simpl in H.
-    destruct (type_of (etvar k e) t) eqn:type_of_body.
-    + inversion H. auto using t_abs_t.
-    + inversion H.
-  - intros. simpl in H.
-    destruct (type_of e t) eqn:?.
-    + destruct t1 eqn:type_of_term.
-      * inversion H.
-      * inversion H.
-      * destruct (kind_of e t0) eqn:kind_of_arg.
-        { destruct (Arith.Compare_dec.leb k0 k) eqn:k0_leb.
-          { inversion H. eapply t_app_t. eauto.
-            eauto using kind_of_correct, leb_complete, kinding_sub, t_app_t. }
-          { inversion H. } }
-        { inversion H. }
-    + inversion H.
-Qed.
+Section Kinding.
+
+  (** This theorem states the correctness of kind_of. That is,
+      that whenever kind_of assigns a kind to a type, this kind
+      is indeed an appropriate kind for the type. *)
+  Theorem kind_of_correct (T : typ) : 
+    forall (e : env) (K : kind), 
+      kind_of e T = Some K -> kinding e T K.
+    induction T.
+    - intros. simpl in H.
+      remember (bwf_env e).
+      destruct b.
+      + apply eq_sym in Heqb. eauto using bwf_env_correct, k_tvar.
+      + discriminate H.
+    - intros. simpl in H.
+      remember (kind_of e T1) as kind_of_T1.
+      remember (kind_of e T2) as kind_of_T2.
+      destruct kind_of_T1, kind_of_T2;
+        [ inversion H; eauto using k_tarr | inversion H .. ].
+    - intros. simpl in H.
+      destruct (kind_of (etvar k e) T) eqn:kind_of_etvar.
+      + inversion H. eauto using k_tall.
+      + inversion H.
+  Qed. 
+
+End Kinding.
+
+Section Typing.
+
+  (** This theorem states the correctness of type_of. That is,
+      that whenever type_of assigns a type to a term, this type
+      is indeed an appropriate type for the term. *)
+  Theorem type_of_correct (t : term) : 
+    forall (e : env) (T : typ), 
+      type_of e t = Some T -> typing e t T.
+    induction t.
+    - intros. simpl in H.
+      destruct (bwf_env e) eqn:env_is_bwf.
+      + auto using t_var, bwf_env_correct.
+      + inversion H.
+    - intros. simpl in H.
+      destruct (type_of (evar t e) t0) eqn:type_of_body.
+      + remember (bwf_typ e t). destruct b.
+        * inversion H. apply t_abs. apply bwf_typ_correct. auto. apply IHt, type_of_body.
+        * discriminate.
+      + inversion H.
+    - intros. simpl in H.
+      destruct (type_of e t1) eqn:type_of_fn.
+      + destruct t.
+        * inversion H.
+        * destruct (type_of e t2) eqn:type_of_arg.
+          { destruct (beq_typ t3 t) eqn:equal_types.
+            { inversion H. rewrite <- H1.
+              eauto. apply beq_typ_correct in equal_types. eapply t_app. eauto. rewrite equal_types. eauto. }
+            { inversion H. } }
+          { inversion H. }
+        * inversion H.
+      + inversion H.
+    - intros. simpl in H.
+      destruct (type_of (etvar k e) t) eqn:type_of_body.
+      + inversion H. auto using t_abs_t.
+      + inversion H.
+    - intros. simpl in H.
+      destruct (type_of e t) eqn:?.
+      + destruct t1 eqn:type_of_term.
+        * inversion H.
+        * inversion H.
+        * destruct (kind_of e t0) eqn:kind_of_arg.
+          { destruct (Arith.Compare_dec.leb k0 k) eqn:k0_leb.
+            { inversion H. eapply t_app_t. eauto.
+              eauto using kind_of_correct, leb_complete, cumulativity, t_app_t. }
+            { inversion H. } }
+          { inversion H. }
+      + inversion H.
+  Qed.
+
+End Typing.
