Makefile
@@ -3,6 +3,9 @@ all: SysF.vo Metatheory.vo Correctness.vo Reduction.vo StrongNormalization.vo
 SysF.vo: SysF.v
 	coqc $<
 
+Correctness.vo: Correctness.v SysF.vo Metatheory.vo
+	coqc $<
+
 StrongNormalization.vo: StrongNormalization.v SysF.vo Reduction.vo Metatheory.vo Correctness.vo
 	coqc $<
 
